sql/init-speech_speakers.sql
@@ -10,4 +10,4 @@ CREATE INDEX IF NOT EXISTS idx_speech_speakers_speech_filename ON speech_speaker
 CREATE INDEX IF NOT EXISTS idx_speech_speakers_speaker_route_pathname ON speech_speakers (speaker_route_pathname);
 
 INSERT OR IGNORE INTO speech_speakers (speech_filename, speaker_route_pathname)
-	VALUES ("2025-11-10-柏林自由會議ai-的角色", "%E5%94%90%E9%B3%B3-3");
+	VALUES ('2025-11-10-柏林自由會議ai-的角色', '%E5%94%90%E9%B3%B3-3');
